cava/experiments/bedrock2/AesProperties.v
@@ -1,0 +1,76 @@
+Require Import Coq.Lists.List.
+Require Import Coq.Strings.String.
+Require Import Coq.ZArith.ZArith.
+Require Import bedrock2.ProgramLogic.
+Require Import bedrock2.Semantics.
+Require Import bedrock2.Syntax.
+Require Import bedrock2.WeakestPrecondition.
+Require Import bedrock2.WeakestPreconditionProperties.
+Require Import coqutil.Word.Interface.
+Require Import coqutil.Map.Interface.
+Require Import coqutil.Tactics.Tactics.
+Require Import Bedrock2Experiments.Aes.
+Import Syntax.Coercions List.ListNotations.
+Local Open Scope Z_scope.
+
+Require Import bedrock2.FE310CSemantics.
+
+SearchHead Semantics.parameters.
+Existing Instances common_h_impl aes_regs_h_impl aes_h_impl.
+
+Section Proofs.
+  Context {fe310_parameters : FE310CSemantics.parameters.parameters}.
+
+  (* For now, empty spec *)
+  Instance spec_of_aes_init : spec_of aes_init :=
+    fun functions =>
+      forall tr mem aes_cfg_operation aes_cfg_mode aes_cfg_key_len aes_ctrl_shadowed_0
+        operation mode_mask mode_offset key_len_mask key_len_offset,
+        isMMIOAddr aes_ctrl_shadowed_0 ->
+        word.unsigned aes_ctrl_shadowed_0 mod 4 = 0 ->
+        let args := [aes_cfg_operation; aes_cfg_mode; aes_cfg_key_len;
+                    aes_ctrl_shadowed_0; operation; mode_mask; mode_offset;
+                    key_len_mask; key_len_offset] in
+        call functions aes_init tr mem args
+             (fun tr m rets => True).
+
+  Lemma aes_init_no_struct_correct :
+    program_logic_goal_for_function! aes_init.
+  Proof.
+    Fail straightline. (* FIXME *)
+    (* This should be a call to [enter], but I got errors from it saying
+       aes_init was not evaluable when it was a bound variable. Unclear why, but
+       I inlined the tactic here and removed the binding *)
+    cbv beta delta [program_logic_goal_for]; intros; bind_body_of_function aes_init;
+    (let fdefn := eval cbv delta [aes_init] in aes_init in
+     let ctx := string2ident.learn fdefn in
+     let H := fresh "_string_to_ident" in
+     pose (H := ctx); lazymatch goal with
+                      | |- ?s _ => cbv beta delta [s]
+                      end).
+
+    (* simplification *)
+    cbv zeta.
+
+    (* (modified) rest of the first straightline clause *)
+    (intros; unfold1_call_goal; cbv beta match delta [call_body];
+     lazymatch goal with
+     | |- if ?test then ?T else _ => replace test with true by reflexivity; change T
+     end; cbv beta match delta [func]).
+
+    (* finally, enter the body of the function *)
+    repeat straightline.
+    eapply interact_nomem; [ solve [repeat straightline] | ].
+    cbn [Semantics.ext_spec ext_spec semantics_parameters].
+    cbv [ext_spec]. rewrite String.eqb_refl.
+    do 2 eexists; ssplit; auto; [ ].
+
+    repeat straightline.
+    eapply interact_nomem; [ solve [repeat straightline] | ].
+    cbn [Semantics.ext_spec ext_spec semantics_parameters].
+    cbv [ext_spec]. rewrite String.eqb_refl.
+    do 2 eexists; ssplit; auto; [ ].
+
+    repeat straightline.
+  Qed.
+End Proofs.
